fix: rest 4 lemma

algorithms/MaxSum.v
@@ -194,6 +194,24 @@ Proof.
       assumption.
 Qed.
 
+Lemma is_indexed_elements_prefix_extend :
+  forall (l : list Z) (x : Z) (s il : list Z),
+    is_indexed_elements l il s ->
+    is_indexed_elements (l ++ [x]) il s.
+Proof.
+  intros l x s il H.
+  unfold is_indexed_elements in *.
+  induction H as [| i a il' s' Hnth Hrest IH]; simpl.
+  - apply Forall2_nil.
+  - apply Forall2_cons.
+    + assert (Hrange: 0 <= i < Zlength l).
+      { apply Znth_error_range in Hnth. tauto. }
+      rewrite (Znth_error_app_l _ _ _ Hrange).
+      exact Hnth.
+    + apply IH.
+Qed.
+
+
 Lemma sincr_extend_last: forall (il: list Z) (last_idx: Z),
   sincr il ->
   (il = [] \/ last il 0 < last_idx) ->
@@ -598,20 +616,15 @@ Proof.
   intros l x s H.
   unfold feasible_set, non_adjacent_subseq in H.
   destruct H as [il [Hidx [Hsincr Hgap]]].   
-  
   destruct (list_snoc_destruct il) as [Heq_il | [i_last [il' Heq_il]]]; subst il.
-  
   - 
     left.
     apply (feasible_set_app_x_inv_empty_il l x s); auto.
-  
   -
     destruct (Z.eq_dec i_last (Zlength l)) as [Heq_idx | Hneq_idx]. 
-    
     + 
       right.
       eapply (feasible_set_app_x_inv_i_last_eq l x s il' i_last); eassumption.
-    
     + 
       left.
       eapply (feasible_set_app_x_inv_i_last_neq l x s il' i_last); eassumption. 
@@ -786,12 +799,150 @@ Proof.
 Qed. 
 
 (** Level 3: Prove that the algorithm returns a correct feasible subsequence achieving the maximum value *)
+Lemma sum_single: forall x, sum [x] = x.
+Proof. intros. simpl. apply Z.add_0_r. Qed.
+
+Lemma sincr_tail: forall a l, sincr (a :: l) -> sincr l.
+Proof.
+  intros a l Hsincr. unfold sincr in *.
+  destruct l as [|b l'].
+  - simpl. auto.
+  - simpl in Hsincr. simpl. inversion Hsincr; subst. assumption.
+Qed.   
+
+Lemma feasible_set_preserved: 
+  forall l s t,
+    feasible_set l t -> feasible_set (l ++ [s]) t.
+Proof.
+  intros l s t [il [Hidx [Hsincr Hgap]]].
+  exists il. split; [| split; auto].
+  - revert s l t Hsincr Hgap Hidx.  
+    induction il as [|i il' IH]; intros s l t Hsincr Hgap Hidx.
+    + inversion Hidx; subst. apply Forall2_nil.
+    + destruct t as [|y t'].
+      * inversion Hidx.
+      * constructor.
+        -- inversion Hidx; subst.
+           assert (H_range: 0 <= i < Zlength l).
+           { apply Znth_error_range in H2. tauto. }
+           rewrite (Znth_error_app_l _ _ _ H_range). apply H2.
+        -- inversion Hidx; subst. apply IH. 
+           ++ apply (sincr_tail i il' Hsincr).
+           ++ intros i0 j0 Hi0 Hj0. apply Hgap.
+              ** right. apply Hi0.
+              ** apply in_cons. apply Hj0.
+           ++ apply H4.                
+Qed.
+
+Lemma last_In: 
+  forall (l: list Z) (tail: Z),
+    l <> [] -> In (last l tail) l.
+Proof. 
+  intros l tail H. induction l as [|a l' IH].
+  - contradiction.
+  - destruct l' as [|a' l''].
+    + simpl. left. reflexivity.
+    + simpl. right. apply IH. discriminate.
+Qed.         
+
+Lemma feasible_set_extend:
+  forall (l: list Z) (s: Z) (t: list Z),
+    feasible_set (removelast l) t -> 
+    feasible_set (l ++ [s]) (t ++ [s]).
+Proof.
+  intros l s t Hfeas. unfold feasible_set, non_adjacent_subseq in Hfeas.
+  destruct Hfeas as [il [Hidx [Hsincr Hgap]]].
+  exists (il ++ [Zlength l]). repeat split. 
+  - apply is_indexed_elements_app.
+    + apply is_indexed_elements_extend. apply Hidx.
+    + apply is_indexed_elements_cons.
+      * apply Znth_error_snoc_last.
+      * apply is_indexed_elements_nil.
+  - apply sincr_extend_last.
+    + apply Hsincr.
+    + destruct il as [|i' il'].
+      * left. reflexivity. 
+      * right. apply is_indexed_elements_range in Hidx. 
+        rewrite Forall_forall in Hidx.
+        assert (Hlast_In: In(last (i' :: il') 0) (i' :: il')).
+        { apply last_In. discriminate. }
+        specialize (Hidx _ Hlast_In).
+        destruct (list_snoc_destruct l) as [Heq_l | [a [l' Heq_l]]].
+        -- subst l; simpl in *; unfold Zlength in *; simpl in *. lia.
+        -- subst l. rewrite removelast_app in Hidx by discriminate.
+           simpl in Hidx. rewrite app_nil_r in Hidx.
+           rewrite Zlength_app. unfold Zlength in *.  simpl. lia.
+  - intros x y Hx Hy. apply in_app_or in Hx. apply in_app_or in Hy.
+    destruct Hx as [Hx_il | Hx_lt]; destruct Hy as [Hy_il | Hy_lt].
+    + apply Hgap; tauto.
+    + simpl in *. destruct Hy_lt as [Heq_y | Hf]; [|contradiction].
+      subst y. apply is_indexed_elements_range in Hidx.
+      rewrite Forall_forall in Hidx. specialize (Hidx _ Hx_il).
+      destruct (list_snoc_destruct l) as [Heq_l | [a [l' Heq_l]]].
+      * subst l. simpl in Hidx. unfold Zlength in *. simpl. lia.
+      * subst l. rewrite removelast_app in Hidx by discriminate.
+        simpl in Hidx. rewrite app_nil_r in Hidx.
+        rewrite Zlength_app. unfold Zlength in *. simpl. lia.
+    + simpl in *. destruct Hx_lt as [Heq_x | Hf]; [|contradiction]. 
+      subst x. apply is_indexed_elements_range in Hidx. 
+      rewrite Forall_forall in Hidx. specialize (Hidx _ Hy_il). 
+      destruct (list_snoc_destruct l) as [Heq_l | [a [l' Heq_l]]]. 
+      * subst l. simpl. unfold Zlength in *. simpl in *. lia.
+      * subst l. rewrite removelast_app in Hidx by discriminate.
+        simpl in Hidx. rewrite app_nil_r in Hidx. 
+        rewrite Zlength_app. unfold Zlength in *. simpl. lia.
+    + simpl in *. destruct Hx_lt as [Heq_x | Hf]; [|contradiction].
+      destruct Hy_lt as [Heq_y | Hf]; [|contradiction]. subst x y. lia.    
+Qed.
+
 Theorem max_sum_full_correct :
   forall l,
     Hoare (max_sum l)
       (fun '(m, s) => max_sum_full_spec l m s).
 Proof.
-Admitted.
+  intros l. unfold max_sum. eapply Hoare_bind.
+  - eapply Hoare_list_iter with 
+      (I := fun done st => 
+              match st with 
+                (m1, ans1, m2, ans2) => 
+                  max_value_spec done m1 /\
+                  max_value_spec (removelast done) m2 /\
+                  feasible_set done ans1 /\ sum ans1 = m1 /\
+                  feasible_set (removelast done) ans2 /\  sum ans2 = m2
+              end).
+    + simpl. repeat split.
+      * apply max_value_spec_nil.
+      * apply max_value_spec_nil.
+      * apply feasible_set_nil_intro.
+      * apply feasible_set_nil_intro.
+    + intros x done st. destruct st as [[[m1 ans1] m2] ans2].
+      intros [Hm1 [Hm2 [Hfeas1 [Hsum1 [Hfeas2 Hsum2]]]]]. apply Hoare_choice.
+      * eapply Hoare_assume_bind. intros H_le. apply Hoare_ret. repeat split. 
+        -- assert (Hmax: max_value_spec (done ++ [x]) (Z.max m1 (m2 + x))).
+           { apply max_value_spec_app; auto. }
+           replace (Z.max m1 (m2 + x)) with (m2 + x) in Hmax.
+           ++ apply Hmax.
+           ++ symmetry. apply Z.max_r. lia.
+        -- rewrite removelast_app_x. apply Hm1.
+        -- apply feasible_set_extend. tauto.
+        -- simpl. rewrite sum_app, sum_single, Hsum2. reflexivity.
+        -- rewrite removelast_app_x. apply Hfeas1.
+        -- apply Hsum1.
+      * eapply Hoare_assume_bind. intros H_ge. apply Hoare_ret. repeat split.
+        -- assert (Hmax: max_value_spec (done ++ [x]) (Z.max m1 (m2 + x))).
+           { apply max_value_spec_app; auto. }
+           replace (Z.max m1 (m2 + x)) with m1 in Hmax.
+           ++ apply Hmax.
+           ++ symmetry. apply Z.max_l. lia.
+        -- rewrite removelast_app_x. apply Hm1.
+        -- apply feasible_set_preserved. assumption.
+        -- assumption.
+        -- rewrite removelast_app_x. apply Hfeas1.
+        -- apply Hsum1.
+  - intros st. destruct st as [[[m1 ans1] m2] ans2].
+    intros [Hm1 [Hm2 [Hfeas1 [Hsum1 [_ _]]]]]. apply Hoare_ret.
+    unfold max_sum_full_spec. repeat split; auto.
+Qed.
 
 (** Lexicographical comparison of index lists *)
 Fixpoint index_lex_lt (il1 il2: list Z) : Prop :=
@@ -841,10 +992,1075 @@ Definition max_sum_lex (l: list Z): program (Z * list Z * list Z) :=
       (0, [], [], 0, [], [], 0);; 
   ret (max1, ans1, il1).
 
+
+Definition max_sum_lex_inv (done : list Z)
+             (max1 : Z) (ans1 : list Z) (il1 : list Z)
+             (max2 : Z) (ans2 : list Z) (il2 : list Z)
+             (idx : Z) : Prop :=
+  Zlength done = idx /\
+  (* ans1 is optimal and lex-min for done *)
+  max_sum_full_spec done max1 ans1 /\
+  is_indexed_elements done il1 ans1 /\
+  non_adjacent_in il1 /\
+  (forall s' il',
+     feasible_set done s' ->
+     is_indexed_elements done il' s' ->
+     non_adjacent_in il' ->
+     sum s' = max1 ->
+     index_lex_lt il1 il' \/ il1 = il') /\
+  (* ans2 is optimal and lex-min for removelast done *)
+  (match done with
+   | [] => max2 = 0 /\ ans2 = [] /\ il2 = []
+   | _ => max_sum_full_spec (removelast done) max2 ans2 /\
+          is_indexed_elements (removelast done) il2 ans2 /\
+          non_adjacent_in il2 /\
+          (forall s' il',
+             feasible_set (removelast done) s' ->
+             is_indexed_elements (removelast done) il' s' ->
+             non_adjacent_in il' ->
+             sum s' = max2 ->
+             index_lex_lt il2 il' \/ il2 = il')
+   end).
+
+Lemma proof_il'_nil :
+  forall (s' il' : list Z)
+    (H : feasible_set [] s')
+    (H0 : is_indexed_elements [] il' s')
+    (H1 : non_adjacent_in il')
+    (H2 : sum s' = 0),
+    [] = il'.
+Proof.
+  intros s' il' H H0 H1 H2.
+  apply feasible_set_nil in H.
+  subst s'.
+  apply is_indexed_elements_nil_inv_r in H0.
+  rewrite H0; reflexivity.
+Qed.
+
+Lemma idx_eq_zero (idx : Z) (Hlen : Zlength ([] : list Z) = idx) : idx = 0.
+Proof.
+  unfold Zlength in Hlen.
+  simpl in Hlen.
+  rewrite Hlen; reflexivity.
+Qed.
+
+Lemma In_0_non_adjacent :
+  forall i j : Z, In i [0] -> In j [0] -> i + 1 <> j.
+Proof.
+  intros. destruct H, H0.
+  ++ lia.
+  ++ simpl in H0. tauto.
+  ++ simpl in H. tauto.
+  ++ simpl in H. tauto.
+Qed.
+
+Lemma is_indexed_elements_restrict :
+  forall (l : list Z) (x : Z) (s il : list Z),
+  is_indexed_elements (l ++ [x]) il s ->
+  (forall i, In i il -> i < Zlength l) ->
+  is_indexed_elements l il s.
+Proof.
+  intros l x s il Hidx Hbound.
+  revert s Hidx.
+  induction il as [|i il' IH]; intros s Hidx; simpl in *.
+  - apply is_indexed_elements_nil_inv_l in Hidx.
+    rewrite Hidx.
+    apply is_indexed_elements_nil.
+  - apply is_indexed_elements_cons_inv_l in Hidx as (a & s' & Hnth & Hrest & ->).
+    apply is_indexed_elements_cons.
+    + (* Goal: Znth_error l i = Some a *)
+      (* From Hnth: Znth_error (l ++ [x]) i = Some a *)
+      pose proof (Znth_error_range _ _ _ Hnth) as [Hge Hlt_full].
+      (* Hbound gives: i < Zlength l *)
+      assert (Hin: In i (i :: il')) by (left; reflexivity).
+      specialize (Hbound i Hin) as Hlt.
+      (* Now we have 0 <= i and i < Zlength l *)
+      rewrite (Znth_error_app_l l [x] i (conj Hge Hlt)) in Hnth.
+      exact Hnth.
+    + (* Inductive step for il' *)
+      apply IH.
+      intros j Hj.
+      apply Hbound.
+      right. exact Hj. tauto.
+Qed.
+
+Lemma max_sum_full_spec_inv :
+  forall (l : list Z) (m : Z) (s : list Z),
+  max_sum_full_spec l m s ->
+  max_value_spec l m /\ feasible_set l s /\ sum s = m.
+Proof.
+  intros l m s H.
+  exact H.
+Qed.
+
+Lemma feasible_single :
+  forall x : Z,
+    feasible_set [x] [x].
+Proof.
+  unfold feasible_set, non_adjacent_subseq.
+  exists [0].
+  split.
+  + unfold is_indexed_elements.
+      constructor; [compute; reflexivity | constructor].
+  + unfold non_adjacent_in; simpl.
+    split; [tauto | intros i j Hi Hj; inversion Hi; inversion Hj; lia].
+Qed.
+
+Lemma Zlength_removelast : forall (A: Type) (l : list A),
+  l <> [] -> Zlength (removelast l) = Zlength l - 1.
+Proof.
+  intros A l Hnonnil.
+  induction l as [| a l'].
+  - exfalso; contradiction.
+  - destruct l' as [| b l''].
+    + simpl removelast. simpl. unfold Zlength. tauto.
+    + simpl removelast in *.
+      assert (Hl'_nonnil : b :: l'' <> []) by (
+        intros H; discriminate H
+      ).
+      rewrite Zlength_cons.
+      rewrite Zlength_cons.
+      rewrite (IHl' Hl'_nonnil).
+      lia.
+Qed.
+
+Lemma in_singleton: forall {A} (a x : A), In x [a] <-> x = a.
+Proof.
+  split; intros H.
+  - now inversion H.
+  - subst; left; reflexivity.
+Qed.
+
+
+Lemma max_value_spec_single_positive :
+  forall x : Z, x > 0 -> max_value_spec [x] x.
+Proof.
+  intros x Hx. left. exists [x]. repeat split.
+  - apply feasible_single.
+  - apply sum_single.
+  - intros t Ht. unfold feasible_set, non_adjacent_subseq in *.
+    destruct Ht as [il [Hidx Hnonadj]].
+    assert (Ht_is_empty_or_x: t = [] \/ t = [x]).
+    { 
+      unfold is_indexed_elements in Hidx. destruct t as [|a t'].
+      + left. auto.
+      + right. apply is_indexed_elements_cons_inv_r in Hidx.
+        destruct Hidx as [i [il' [Heq [Hnth Hrest]]]].
+        assert (Hi: i = 0).
+        { 
+          apply Znth_error_range in Hnth. unfold Zlength in Hnth. simpl in Hnth. lia. 
+        }
+        subst i. assert (Ha: a = x).
+        {
+          assert (Hx_nth: Znth_error [x] 0 = Some x) by apply Znth_error_cons_0. 
+          rewrite Hx_nth in Hnth. injection Hnth as Ha. symmetry. apply Ha.
+        }
+        subst a. assert (Ht'_nil: t' = []).
+        {
+          destruct t' as [|b t''].
+          - reflexivity. 
+          - exfalso. apply is_indexed_elements_cons_inv_r in Hrest.
+            destruct Hrest as [j [il'' [Heq_il' [Hnth' Hrest']]]].
+            apply Znth_error_range in Hnth'. simpl in Hnth'.
+            destruct Hnonadj as [Hsincr _]. rewrite Heq in Hsincr.
+            apply sincr_cons_tail_Forall_lt in Hsincr. rewrite Heq_il' in Hsincr.
+            assert (Hj_in: In j (j :: il'')) by (left;reflexivity).
+            assert (Hj_0: j = 0) by (unfold Zlength in Hnth'; simpl in Hnth'; lia).  
+            rewrite Hj_0 in Hsincr.
+            apply Forall_cons_iff in Hsincr.
+            destruct Hsincr as [H0 _].
+            lia.
+        }
+        rewrite Ht'_nil.
+        reflexivity. 
+    }
+    destruct Ht_is_empty_or_x.
+    + rewrite H; simpl; lia.
+    + rewrite H; simpl; lia.
+Qed.
+
+(* 此时 x>0, 取x最大 *)
+Lemma max_sum_lex_inv_single_positive :
+  forall (l : list Z) (x : Z)
+    (Hfull1 : max_sum_full_spec [] 0 [])
+    (Hgap1 : non_adjacent_in [])
+    (Hgt : x > 0)
+    (Hlex1 : forall s' il',
+               feasible_set [] s' ->
+               is_indexed_elements [] il' s' ->
+               non_adjacent_in il' -> sum s' = 0 ->
+               index_lex_lt [] il' \/ [] = il')
+    (Hidx0 : Zlength ([] : list Z) = 0),
+  max_sum_lex_inv [x] x [x] [0] 0 [] [] 1.
+Proof.
+  intros l x Hfull1 Hgap1 Hgt Hlex1 Hidx0.
+  unfold max_sum_lex_inv.
+  repeat split.
+  - apply max_value_spec_single_positive; tauto.
+  - apply feasible_single.
+  - apply sum_single.
+  - (* is_indexed_elements [x] [0] [x] *)
+    unfold is_indexed_elements.
+    apply Forall2_cons.
+    + simpl; reflexivity.
+    + apply Forall2_nil.
+  - apply In_0_non_adjacent.
+  - intros s' il' Hfeas Hidx Hnonadj Hsum.
+    change ([x]) with ([] ++ [x]) in Hfeas.
+    apply feasible_set_app_x_inv in Hfeas as [Hl | [t' [Heq Ht']]].
+    + exfalso. apply feasible_set_nil in Hl; subst s'. simpl in Hsum. lia.
+    + subst s'. apply feasible_set_nil in Ht'; subst t'.
+      simpl in Hidx.
+      apply is_indexed_elements_cons_inv_r in Hidx.
+      destruct Hidx as (i & il'' & Heq_il & Hnth & Hnil).
+      subst il'.
+      apply is_indexed_elements_nil_inv_r in Hnil; subst il''.
+      apply Znth_error_range in Hnth.
+      simpl in Hnth. assert (i = 0). { destruct Hnth; unfold Zlength in H0; simpl in H0; lia. }
+      subst i.
+      right. reflexivity.
+  - simpl. apply max_value_spec_nil.
+  - simpl. apply feasible_set_nil_intro.
+  - simpl. apply is_indexed_elements_nil.
+  - tauto.
+  - apply Hlex1.
+Qed.
+
+(* 此时 x < max1 = 0, 不取就是最大 *)
+Lemma max_sum_lex_inv_single_case :
+  forall (l : list Z) (x max1 idx : Z) (ans1 il1 : list Z)
+    (Hlen : Zlength ([] : list Z) = idx)
+    (Hfull1 : max_sum_full_spec [] max1 ans1)
+    (Hidx1 : is_indexed_elements [] il1 ans1)
+    (Hgap1 : non_adjacent_in il1)
+    (Hlex1 : forall s' il',
+               feasible_set [] s' ->
+               is_indexed_elements [] il' s' ->
+               non_adjacent_in il' -> sum s' = max1 ->
+               index_lex_lt il1 il' \/ il1 = il')
+    (Hlt : x < max1),
+  max_sum_lex_inv [x] max1 ans1 il1 max1 ans1 il1 (idx + 1).
+Proof.
+  intros l x max1 idx ans1 il1 Hlen Hfull1 Hidx1 Hgap1 Hlex1 Hlt.
+  unfold max_sum_lex_inv.
+  repeat split.
+
+  - simpl in Hlen; unfold Zlength in Hlen; simpl in Hlen; rewrite <- Hlen; reflexivity.
+  - pose proof (proj1 (proj2 Hfull1)) as Hfeas_ans.
+    pose proof (proj2 (proj2 Hfull1)) as Hsum_ans.
+    apply feasible_set_nil in Hfeas_ans. rewrite Hfeas_ans in Hsum_ans.
+    simpl in Hsum_ans.  (* Hsum_ans : 0 = max1 *)
+    subst max1.
+    (* Now prove max_value_spec [x] 0 *)
+    right.
+    split.
+    + intros s Hfeas.
+      change ([x]) with ([] ++ [x]) in Hfeas.
+      apply feasible_set_app_x_inv in Hfeas as [Hl | [t' [Heq Ht']]].
+      * (* s feasible in [] => s = [] => sum = 0 *)
+        apply feasible_set_nil in Hl; subst s; simpl; lia.
+      * (* s = t' ++ [x], t' feasible in [] => t' = [], s = [x] *)
+        apply feasible_set_nil in Ht'; subst t'. simpl in Heq; subst s.
+        simpl. lia.  (* x < 0, so sum = x < 0 <= 0 *)
+    + reflexivity.
+  - (* feasible_set [x] ans1 *)
+    apply max_sum_full_spec_inv in Hfull1 as [_ [Hfeas _]].
+    apply feasible_set_nil in Hfeas; subst ans1.
+    unfold feasible_set. unfold non_adjacent_subseq. exists []. split.
+    * apply is_indexed_elements_nil.
+    * unfold non_adjacent_in. split.
+      -- unfold sincr. tauto.
+      -- intros i j Hini Hinj. destruct Hini, Hinj.
+  - apply (proj2 (proj2 Hfull1)).
+  - (* is_indexed_elements [x] il1 ans1 *)
+    apply max_sum_full_spec_inv in Hfull1 as [_ [Hfeas _]].
+    apply feasible_set_nil in Hfeas; subst ans1.
+    apply is_indexed_elements_nil_inv_r in Hidx1; subst il1.
+    apply is_indexed_elements_nil.
+  - apply (proj1 Hgap1).
+  - apply (proj2 Hgap1).
+  - (* lex min for [x] *)
+    intros s' il' Hfeas Hidx Hnonadj Hsum.
+    (* Extract ans1 = [], max1 = 0 *)
+    pose proof (proj1 (proj2 Hfull1)) as Hfeas_ans.
+    pose proof (proj2 (proj2 Hfull1)) as Hsum_ans.
+    apply feasible_set_nil in Hfeas_ans; subst ans1.
+    simpl in Hsum_ans.  (* Hsum_ans : 0 = max1 *)
+    rewrite <- Hsum_ans in Hsum.   (* sum s' = 0 *)
+    rewrite <- Hsum_ans in Hlt.    (* x < 0 *)
+    change ([x]) with ([] ++ [x]) in Hfeas.
+    apply feasible_set_app_x_inv in Hfeas as [Hl | [t' [Heq Ht']]].
+    + (* s' = [] *)
+      apply feasible_set_nil in Hl; subst s'.
+      apply is_indexed_elements_nil_inv_r in Hidx; subst il'.
+      apply is_indexed_elements_nil_inv_r in Hidx1; subst il1.
+      right. reflexivity.
+    + (* s' = t' ++ [x] *)
+      apply feasible_set_nil in Ht'; subst t'.
+      subst s'. simpl in Hsum.  (* Hsum : x = 0 *)
+      lia.  (* x = 0 and x < 0 → contradiction *)
+  - (* max_value_spec [] max1 *)
+    simpl. apply (proj1 Hfull1).
+  - (* feasible_set [] ans1 *)
+    apply (proj1 (proj2 Hfull1)).
+  - (* sum ans1 = max1 *)
+    apply (proj2 (proj2 Hfull1)).
+  - (* is_indexed_elements [] il1 ans1 *)
+    apply Hidx1.
+  - (* sincr il1 *)
+    apply (proj1 Hgap1).
+  - (* non-adjacent gap *)
+    apply (proj2 Hgap1).
+  - (* lex min for [] *)
+    apply Hlex1.
+Qed.
+
+(* Hlt 矛盾 *)
+Lemma max_sum_lex_inv_contradiction_case :
+  forall (l : list Z) (x max1 idx : Z) (ans1 il1 : list Z)
+    (Hlen : Zlength ([] : list Z) = idx)
+    (Hfull1 : max_sum_full_spec [] max1 ans1)
+    (Hidx1 : is_indexed_elements [] il1 ans1)
+    (Hgap1 : non_adjacent_in il1)
+    (Hlex1 : forall s' il',
+               feasible_set [] s' ->
+               is_indexed_elements [] il' s' ->
+               non_adjacent_in il' -> sum s' = max1 ->
+               index_lex_lt il1 il' \/ il1 = il')
+    (Heq : x = max1)
+    (Hlt : index_lex_lt ([] ++ [idx]) il1),
+  max_sum_lex_inv [x] x [x] [idx] max1 ans1 il1 (idx + 1).
+Proof.
+  intros l x max1 idx ans1 il1 Hlen Hfull1 Hidx1 Hgap1 Hlex1 Heq Hlt.
+  unfold max_sum_lex_inv.
+  repeat split.
+
+  - simpl in Hlen; unfold Zlength in Hlen; simpl in Hlen; rewrite <- Hlen; reflexivity.
+  - pose proof (proj1 (proj2 Hfull1)) as Hfeas_ans.
+    pose proof (proj2 (proj2 Hfull1)) as Hsum_ans.
+    apply feasible_set_nil in Hfeas_ans. rewrite Hfeas_ans in Hsum_ans.
+    simpl in Hsum_ans.  (* Hsum_ans : 0 = max1 *)
+    subst max1.
+    (* Now prove max_value_spec [x] 0 *)
+    right.
+    split.
+    + intros s Hfeas.
+      change ([x]) with ([] ++ [x]) in Hfeas.
+      apply feasible_set_app_x_inv in Hfeas as [Hl | [t' [Heq Ht']]].
+      * (* s feasible in [] => s = [] => sum = 0 *)
+        apply feasible_set_nil in Hl; subst s; simpl; lia.
+      * (* s = t' ++ [x], t' feasible in [] => t' = [], s = [x] *)
+        apply feasible_set_nil in Ht'; subst t'. simpl in Heq; subst s.
+        simpl. lia.  (* x < 0, so sum = x < 0 <= 0 *)
+    + rewrite Hsum_ans. reflexivity.
+  - apply feasible_single.
+  - apply sum_single.
+  - unfold is_indexed_elements.
+    simpl in Hlen; unfold Zlength in Hlen; simpl in Hlen.
+    constructor.
+    + rewrite <- Hlen. reflexivity.
+    + constructor.
+  - intros i j Hini Hinj. destruct Hini, Hinj.
+    + lia.
+    + simpl in H0; tauto.
+    + simpl in H; tauto.
+    + simpl in H; tauto.
+  - intros s' il' Hfeas Hidx Hnonadj Hsum.
+    (* First, get ans1 = [] *)
+    pose proof (proj1 (proj2 Hfull1)) as Hfeas_ans.
+    apply feasible_set_nil in Hfeas_ans; subst ans1.
+    change ([x]) with ([] ++ [x]) in Hfeas.
+    apply feasible_set_app_x_inv in Hfeas as [Hl | [t' [Heq_s Ht']]].
+    + (* s' = [] *)
+      apply feasible_set_nil in Hl; subst s'.
+      apply is_indexed_elements_nil_inv_r in Hidx; subst il'.
+      (* Now Hidx1 : is_indexed_elements [] il1 [] *)
+      apply is_indexed_elements_nil_inv_r in Hidx1; subst il1.
+      left. exact Hlt.
+    + (* s' = [x] *)
+      pose proof (proj2 (proj2 Hfull1)) as Hsum_ans.
+      simpl in Hsum_ans. rewrite <- Heq in Hsum_ans.  (* x = 0 *)
+      apply feasible_set_nil in Ht'; subst t'. subst s'.
+      apply is_indexed_elements_cons_inv_r in Hidx.
+      destruct Hidx as (i & il'' & Heq_il & Hnth & Hnil).
+      subst il'.
+      apply is_indexed_elements_nil_inv_r in Hnil; subst il''.
+      apply Znth_error_range in Hnth.
+      simpl in Hnth. assert (i = 0). { destruct Hnth; unfold Zlength in H0; simpl in H0; lia. }
+      subst i.
+      simpl in Hlen; unfold Zlength in Hlen; simpl in Hlen.
+      rewrite Hlen.
+      right. reflexivity.
+- simpl. apply (proj1 Hfull1).
+- apply (proj1 (proj2 Hfull1)).
+- apply (proj2 (proj2 Hfull1)).
+- apply Hidx1.
+- apply (proj1 Hgap1).
+- apply (proj2 Hgap1).
+- apply Hlex1.
+Qed.
+
+Lemma max_sum_lex_inv_valid_case :
+  forall (l : list Z) (x max1 idx : Z) (ans1 il1 : list Z)
+    (Hlen : Zlength ([] : list Z) = idx)
+    (Hfull1 : max_sum_full_spec [] max1 ans1)
+    (Hidx1 : is_indexed_elements [] il1 ans1)
+    (Hgap1 : non_adjacent_in il1)
+    (Hlex1 : forall s' il',
+               feasible_set [] s' ->
+               is_indexed_elements [] il' s' ->
+               non_adjacent_in il' -> sum s' = max1 ->
+               index_lex_lt il1 il' \/ il1 = il')
+    (Heq : x = max1)
+    (Hnlt : ~ index_lex_lt ([] ++ [idx]) il1),
+  max_sum_lex_inv [x] max1 ans1 il1 max1 ans1 il1 (idx + 1).
+Proof.
+  intros l x max1 idx ans1 il1 Hlen Hfull1 Hidx1 Hgap1 Hlex1 Heq Hnlt.
+  unfold max_sum_lex_inv.
+  repeat split.
+  - simpl in Hlen; unfold Zlength in Hlen; simpl in Hlen; rewrite <- Hlen; reflexivity.
+  - pose proof (proj1 (proj2 Hfull1)) as Hfeas.
+    pose proof (proj2 (proj2 Hfull1)) as Hsum.
+    apply feasible_set_nil in Hfeas.
+    subst ans1.
+    simpl in Hsum.
+    subst max1.
+    right; split.
+    + intros s Hfeas_s.
+      change ([x]) with ([] ++ [x]) in Hfeas_s.
+      apply feasible_set_app_x_inv in Hfeas_s as [Hl | [t' [Heq Ht']]].
+      * apply feasible_set_nil in Hl; subst s; simpl; lia.
+      * apply feasible_set_nil in Ht'; subst t'; subst s; simpl; lia.
+    + rewrite Hsum; reflexivity.
+  - (* Goal 3: feasible_set [x] ans1 *)
+    pose proof (proj1 (proj2 Hfull1)) as Hfeas.
+    apply feasible_set_nil in Hfeas; subst ans1.
+    unfold feasible_set. unfold non_adjacent_subseq. exists []. split.
+    + apply is_indexed_elements_nil.
+    + unfold non_adjacent_in; split.
+      * unfold sincr; tauto.
+      * intros i j Hini Hinj. destruct Hini, Hinj.
+  - (* Goal 4: sum ans1 = max1 *)
+    pose proof (proj1 (proj2 Hfull1)) as Hfeas.
+    pose proof (proj2 (proj2 Hfull1)) as Hsum.
+    apply feasible_set_nil in Hfeas; subst ans1.
+    apply Hsum.
+  - (* Goal 5: is_indexed_elements [x] il1 ans1 *)
+    pose proof (proj1 (proj2 Hfull1)) as Hfeas.
+    apply feasible_set_nil in Hfeas. subst ans1.
+    apply is_indexed_elements_nil_inv_r in Hidx1. subst il1.
+    apply is_indexed_elements_nil.
+  - (* Goal 6: sincr il1 *)
+    pose proof (proj1 (proj2 Hfull1)) as Hfeas_ans.
+    apply feasible_set_nil in Hfeas_ans. subst ans1.
+    pose proof (proj2 (proj2 Hfull1)) as Hsum_ans. simpl in Hsum_ans. subst max1.
+    apply is_indexed_elements_nil_inv_r in Hidx1. subst il1. unfold sincr; tauto.
+  - (* Goal 7: gap condition *)
+    pose proof (proj1 (proj2 Hfull1)) as Hfeas_ans.
+    apply feasible_set_nil in Hfeas_ans. subst ans1.
+    apply is_indexed_elements_nil_inv_r in Hidx1; subst il1.
+    intros i j Hi Hj; contradiction.
+  - (* Goal 8: lex min for [x] *)
+    pose proof (proj1 (proj2 Hfull1)) as Hfeas.
+    pose proof (proj2 (proj2 Hfull1)) as Hsum.
+    apply feasible_set_nil in Hfeas; subst ans1.
+    simpl in Hsum; subst max1.
+    apply is_indexed_elements_nil_inv_r in Hidx1; subst il1.
+    intros s' il' Hfeas' Hidx' Hnonadj' Hsum'.
+    change ([x]) with ([] ++ [x]) in Hfeas'.
+    apply feasible_set_app_x_inv in Hfeas' as [Hl | [t' [Heq_s Ht']]].
+    + apply feasible_set_nil in Hl; subst s'.
+      apply is_indexed_elements_nil_inv_r in Hidx'; subst il'.
+      right; reflexivity.
+    + apply feasible_set_nil in Ht'; subst t'; subst s'.
+      apply is_indexed_elements_cons_inv_r in Hidx'.
+      destruct Hidx' as (i & il'' & -> & Hnth & Hnil).
+      apply is_indexed_elements_nil_inv_r in Hnil; subst il''.
+      apply Znth_error_range in Hnth.
+      assert (i = 0) by (destruct Hnth; unfold Zlength in *; simpl in *; lia).
+      subst i.
+      left; simpl; auto.
+  - (* Goal 9: max_value_spec (removelast [x]) max1 *)
+    pose proof (proj1 (proj2 Hfull1)) as Hfeas.
+    apply feasible_set_nil in Hfeas. subst ans1.
+    pose proof (proj2 (proj2 Hfull1)) as Hsum.
+    simpl in Hsum. subst max1.
+    assert (removelast [x] = []) by reflexivity. subst.
+    apply max_value_spec_nil.
+  - (* Goal 10: feasible_set (removelast [x]) ans1 *)
+    pose proof (proj1 (proj2 Hfull1)) as Hfeas.
+    apply feasible_set_nil in Hfeas; subst ans1.
+    apply feasible_set_nil_intro.
+  - (* Goal 11: sum ans1 = max1 *)
+    exact (proj2 (proj2 Hfull1)).
+  - (* Goal 12: is_indexed_elements (removelast [x]) il1 ans1 *)
+    pose proof (proj1 (proj2 Hfull1)) as Hfeas.
+    apply feasible_set_nil in Hfeas. subst ans1.
+    apply is_indexed_elements_nil_inv_r in Hidx1; subst il1.
+    pose proof (proj1 (proj2 Hfull1)) as Hfeas.
+    apply feasible_set_nil in Hfeas.
+    apply is_indexed_elements_nil.
+  - (* Goal 13: sincr il1 *)
+    pose proof (proj1 (proj2 Hfull1)) as Hfeas.
+    apply feasible_set_nil in Hfeas. subst ans1.
+    apply is_indexed_elements_nil_inv_r in Hidx1; subst il1.
+    simpl; auto.
+  - (* Goal 14: gap condition *)
+    pose proof (proj1 (proj2 Hfull1)) as Hfeas.
+    apply feasible_set_nil in Hfeas. subst ans1.
+    apply is_indexed_elements_nil_inv_r in Hidx1; subst il1.
+    intros i j Hi Hj; contradiction.
+  - (* Goal 15: lex min for removelast [x] = [] *)
+    pose proof (proj1 (proj2 Hfull1)) as Hfeas.
+    apply feasible_set_nil in Hfeas; subst ans1.
+    apply is_indexed_elements_nil_inv_r in Hidx1; subst il1.
+    pose proof (proj2 (proj2 Hfull1)) as Hsum.
+    simpl in Hsum; subst max1.
+    intros s' il' Hfeas' Hidx' Hnonadj' Hsum'.
+    apply feasible_set_nil in Hfeas'; subst s'.
+    apply is_indexed_elements_nil_inv_r in Hidx'; subst il'.
+    right; reflexivity.
+Qed.
+
+Lemma index_lex_lt_extend_app_both :  
+  forall (d0 x max1 max2 idx : Z) (drest ans2 il2 : list Z) (s' il' : list Z),
+    Zlength (d0 :: drest) = idx ->
+    max_sum_full_spec (removelast (d0 :: drest)) max2 ans2 ->
+    is_indexed_elements (removelast (d0 :: drest)) il2 ans2 ->
+    non_adjacent_in il2 ->
+    (forall s' il',
+       feasible_set (removelast (d0 :: drest)) s' ->
+       is_indexed_elements (removelast (d0 :: drest)) il' s' ->
+       non_adjacent_in il' -> sum s' = max2 ->
+       index_lex_lt il2 il' \/ il2 = il') ->
+    max2 + x > max1 ->
+    feasible_set ((d0 :: drest) ++ [x]) s' ->
+    is_indexed_elements ((d0 :: drest) ++ [x]) il' s' ->
+    non_adjacent_in il' ->
+    sum s' = max2 + x ->
+    index_lex_lt (il2 ++ [idx]) il' \/ il2 ++ [idx] = il'.  
+Proof.
+Admitted.
+
+Lemma max_sum_lex_inv_extend_case :
+  forall (d0 x max1 max2 idx : Z) (drest ans1 il1 ans2 il2 : list Z)
+    (Hlen : Zlength (d0 :: drest) = idx)
+    (Hfull1 : max_sum_full_spec (d0 :: drest) max1 ans1)
+    (Hidx1 : is_indexed_elements (d0 :: drest) il1 ans1)
+    (Hgap1 : non_adjacent_in il1)
+    (Hlex1 : forall s' il',
+               feasible_set (d0 :: drest) s' ->
+               is_indexed_elements (d0 :: drest) il' s' ->
+               non_adjacent_in il' -> sum s' = max1 ->
+               index_lex_lt il1 il' \/ il1 = il')
+    (Hfull2 : max_sum_full_spec (removelast (d0 :: drest)) max2 ans2)
+    (Hidx2 : is_indexed_elements (removelast (d0 :: drest)) il2 ans2)
+    (Hgap2 : non_adjacent_in il2)
+    (Hlex2 : forall s' il',
+               feasible_set (removelast (d0 :: drest)) s' ->
+               is_indexed_elements (removelast (d0 :: drest)) il' s' ->
+               non_adjacent_in il' -> sum s' = max2 ->
+               index_lex_lt il2 il' \/ il2 = il')
+    (Hgt : max2 + x > max1),
+  max_sum_lex_inv ((d0 :: drest) ++ [x]) (max2 + x) (ans2 ++ [x]) (il2 ++ [idx]) max1 ans1 il1 (idx + 1).
+Proof.
+  intros d0 x max1 max2 idx drest ans1 il1 ans2 il2 Hlen Hfull1 Hidx1 Hgap1 Hlex1 Hfull2 Hidx2 Hgap2 Hlex2 Hgt.
+  unfold max_sum_lex_inv.
+  repeat split.
+
+  - rewrite Zlength_app. rewrite Hlen. reflexivity.
+  - (* Goal2 max_value_spec ((d0 :: drest) ++ [x]) (max2 + x) *)
+    left.
+    exists (ans2 ++ [x]).
+    split.
+    + apply feasible_set_extend.
+      apply (proj1 (proj2 Hfull2)).
+    + split.
+      * rewrite sum_app, sum_single.
+        rewrite (proj2 (proj2 Hfull2)). reflexivity.
+      * intros t Hfeas.
+        apply feasible_set_app_x_inv in Hfeas as [Hleft | [t1 [-> Ht1]]].
+        -- pose proof (proj1 Hfull1) as Hspec1.
+           destruct Hspec1 as [Hexists | [Hle_all Hmax0]].
+           ++ destruct Hexists as (s0 & Hfeas0 & Hsum0 & Hbound).
+              specialize (Hbound t Hleft). lia.
+           ++ specialize (Hle_all t Hleft). lia.
+        -- pose proof (proj1 Hfull2) as Hspec2.
+           destruct Hspec2 as [Hexists | [Hle_all Hmax0]].
+           ++ destruct Hexists as (s2 & Hfeas2 & Hsum2 & Hbound).
+              specialize (Hbound t1 Ht1). rewrite sum_app. simpl; lia.
+           ++ specialize (Hle_all t1 Ht1). rewrite sum_app. simpl; lia.
+  - apply feasible_set_extend.
+    apply (proj1 (proj2 Hfull2)).
+  - rewrite sum_app, sum_single.
+    rewrite (proj2 (proj2 Hfull2)). reflexivity.
+  - apply is_indexed_elements_app.
+    + apply is_indexed_elements_extend.
+      exact Hidx2.
+    + apply is_indexed_elements_cons.
+      * rewrite <- Hlen. apply Znth_error_snoc_last.
+      * apply is_indexed_elements_nil.
+  - apply sincr_extend_last.
+    + apply (proj1 Hgap2).
+    + destruct il2 as [|i0 il2'].
+      * left; reflexivity.
+      * right.
+        assert (Hrem_len: Zlength (removelast (d0 :: drest)) = Zlength (d0 :: drest) - 1).
+        { apply Zlength_removelast. discriminate. }
+        pose proof (is_indexed_elements_range _ _ _ Hidx2) as Hrange_full.
+        rewrite Forall_forall in Hrange_full.
+        assert (Hlast_in: In (last (i0 :: il2') 0) (i0 :: il2')) by (apply last_In; discriminate).
+        specialize (Hrange_full _ Hlast_in).
+        (* Now: last ... < Zlength (removelast (d0::drest)) = Zlength (d0::drest) - 1 = idx - 1 *)
+        rewrite Hrem_len in Hrange_full.
+        rewrite Hlen in Hrange_full.  (* Zlength (d0::drest) = idx *)
+        lia.
+  - intros i j Hi Hj.
+    apply in_app_or in Hi.
+    apply in_app_or in Hj.
+    destruct Hi as [Hi_il2 | Hi_idx]; destruct Hj as [Hj_il2 | Hj_idx].
+    + (* i, j in il2 *)
+      apply (proj2 Hgap2); auto.
+    + assert (Hj_eq: j = idx).
+      { apply in_singleton in Hj_idx. exact Hj_idx. }
+      subst j.
+      assert (Hrem_len: Zlength (removelast (d0 :: drest)) = Zlength (d0 :: drest) - 1).
+      { unfold Zlength; destruct drest. simpl. reflexivity. apply Zlength_removelast. discriminate. }
+      pose proof (is_indexed_elements_range _ _ _ Hidx2) as Hrange.
+      rewrite Forall_forall in Hrange.
+      specialize (Hrange i Hi_il2).
+      rewrite Hrem_len in Hrange.
+      rewrite Hlen in Hrange.
+      lia.
+    + (* i = idx, j in il2 *)
+      assert (Hi_eq: i = idx) by (apply in_singleton in Hi_idx; exact Hi_idx).
+      subst i.
+      assert (Hrem_len: Zlength (removelast (d0 :: drest)) = Zlength (d0 :: drest) - 1).
+      { apply Zlength_removelast. discriminate. }
+      pose proof (is_indexed_elements_range _ _ _ Hidx2) as Hrange.
+      rewrite Forall_forall in Hrange.
+      specialize (Hrange j Hj_il2).
+      rewrite Hrem_len, Hlen in Hrange.
+      lia.
+    + (* i = idx, j = idx *)
+      assert (Hi_eq: i = idx) by (apply in_singleton in Hi_idx; exact Hi_idx).
+      assert (Hj_eq: j = idx) by (apply in_singleton in Hj_idx; exact Hj_idx).
+      subst i j.
+      lia.
+  - intros s' il' Hfeas Hidx' Hnonadj Hsum. 
+    assert (Hfeas_backup : feasible_set ((d0 :: drest) ++ [x]) s') by exact Hfeas.
+    apply feasible_set_app_x_inv in Hfeas as [Hleft | [t' [Heq Ht']]].
+    + exfalso.
+      assert (Hle: sum s' <= max1).
+      { destruct (proj1 Hfull1) as [Hcase1 | Hcase2].   
+        - destruct Hcase1 as (s0 & Hfeas0 & Hsum0 & Hbound).
+          apply Hbound; exact Hleft.
+        - destruct Hcase2 as (Hle_all & Hmax0).
+          rewrite Hmax0.
+          apply Hle_all; exact Hleft. 
+      }
+      lia. 
+    + apply (index_lex_lt_extend_app_both d0 x max1 max2 idx drest ans2 il2 s' il' 
+               Hlen Hfull2 Hidx2 Hgap2 Hlex2 Hgt Hfeas_backup Hidx' Hnonadj Hsum).
+  - rewrite removelast_app_x. apply (proj1 Hfull1).
+  - rewrite removelast_app_x. apply (proj1 (proj2 Hfull1)).
+  - apply (proj2 (proj2 Hfull1)).
+  - rewrite removelast_app_x. exact Hidx1.
+  - apply (proj1 Hgap1).
+  - apply (proj2 Hgap1).
+  - rewrite removelast_app_x. exact Hlex1.
+Qed.
+
+Lemma index_lex_preserve_when_extend_list :
+  forall (l :  list Z) (x : Z) (s' il' il1 ans1 : list Z) (max1 :  Z),
+    l <> [] ->
+    max_sum_full_spec l max1 ans1 ->
+    is_indexed_elements l il1 ans1 ->
+    non_adjacent_in il1 ->
+    (forall s' il',
+       feasible_set l s' ->
+       is_indexed_elements l il' s' ->
+       non_adjacent_in il' ->
+       sum s' = max1 ->
+       index_lex_lt il1 il' \/ il1 = il') ->
+    feasible_set l s' ->
+    is_indexed_elements (l ++ [x]) il' s' ->
+    non_adjacent_in il' ->
+    sum s' = max1 ->
+    index_lex_lt il1 il' \/ il1 = il'.
+Proof. 
+Admitted.
+
+Lemma max_sum_lex_inv_preserve_when_not_taken :
+  forall (l : list Z) (x max1 max2 : Z) (ans1 ans2 il1 : list Z),
+    l <> [] ->
+    max_sum_full_spec l max1 ans1 ->
+    is_indexed_elements l il1 ans1 ->
+    non_adjacent_in il1 ->
+    (forall s' il',
+       feasible_set l s' ->
+       is_indexed_elements l il' s' ->
+       non_adjacent_in il' ->
+       sum s' = max1 ->
+       index_lex_lt il1 il' \/ il1 = il') ->
+    max_sum_full_spec (removelast l) max2 ans2 ->
+    max2 + x < max1 ->
+    max_sum_lex_inv (l ++ [x]) max1 ans1 il1 max1 ans1 il1 (Zlength l + 1).
+Proof.
+  intros l x max1 max2 ans1 ans2 il1 Hneq Hfull1 Hidx1 Hgap1 Hlex1 Hfull2 Hlt.
+  unfold max_sum_lex_inv.
+  repeat split. 
+
+  - apply Zlength_app.
+  - assert (Hspec1: max_value_spec l max1) by (apply (proj1 Hfull1)).
+    assert (Hspec2: max_value_spec (removelast l) max2) by (apply (proj1 Hfull2)).
+    assert (Hspec_app: max_value_spec (l ++ [x]) (Z.max max1 (max2 + x))).
+    { apply max_value_spec_app. exact Hspec1. exact Hspec2. }
+    replace (Z.max max1 (max2 + x)) with max1 in Hspec_app. 
+    + exact Hspec_app.
+    + symmetry. apply Z.max_l. lia.
+  - apply feasible_set_app_x_l. 
+    apply (proj1 (proj2 Hfull1)).
+  - apply (proj2 (proj2 Hfull1)).
+  - apply is_indexed_elements_prefix_extend.
+    tauto.
+  - apply (proj1 Hgap1).
+  - apply (proj2 Hgap1).
+  - intros s' il' Hfeas Hidx' Hnonadj Hsum.
+    apply feasible_set_app_x_inv in Hfeas as [Hfeas_l | [t' [Heq Ht']]].
+    + (* s' 是 l 的可行解 *)
+      apply (index_lex_preserve_when_extend_list l x s' il' il1 ans1 max1 
+               Hneq Hfull1 Hidx1 Hgap1 Hlex1 Hfeas_l Hidx' Hnonadj Hsum).
+    + (* s' = t' ++ [x] *)
+      exfalso.
+      assert (Hsum_t': sum t' <= max2).
+      {
+        pose proof (proj1 Hfull2) as Hspec2.
+        destruct Hspec2 as [Hexists | [Hle Hm0]].
+        - destruct Hexists as (s0 & _ & _ & Hbound).
+          apply Hbound; exact Ht'. 
+        - pose proof Hle t' Ht'. rewrite <- Hm0 in H. apply H.
+      }
+      rewrite Heq in Hsum. pose proof sum_app t' [x].
+      rewrite H in Hsum. simpl in Hsum. lia.
+  - rewrite removelast_app_x by (discriminate Hneq).
+    destruct l as [|a l'].
+    + tauto.
+    + simpl. 
+      repeat split; auto. 
+      unfold max_sum_full_spec in Hfull1.
+      * destruct Hfull1 as [H1 [_ _]]; tauto.
+      * destruct Hfull1 as [_ [H2 _]]; tauto.
+      * destruct Hfull1 as [_ [_ H3]]; tauto. 
+      * unfold non_adjacent_in in Hgap1; destruct Hgap1; tauto.
+      * unfold non_adjacent_in in Hgap1. apply Hgap1.
+Qed.
+
+Lemma index_lex_preserve_eq_case :
+  forall (d0 x :  Z) (drest ans1 il1 ans2 il2 : list Z) (max1 max2 idx : Z)
+    (s' il' : list Z),
+    Zlength (d0 :: drest) = idx ->
+    max_sum_full_spec (d0 :: drest) max1 ans1 ->
+    is_indexed_elements (d0 :: drest) il1 ans1 ->
+    non_adjacent_in il1 ->
+    (forall s' il',
+       feasible_set (d0 :: drest) s' ->
+       is_indexed_elements (d0 :: drest) il' s' ->
+       non_adjacent_in il' -> sum s' = max1 ->
+       index_lex_lt il1 il' \/ il1 = il') ->
+    max_sum_full_spec (removelast (d0 :: drest)) max2 ans2 ->
+    is_indexed_elements (removelast (d0 :: drest)) il2 ans2 ->
+    non_adjacent_in il2 ->
+    (forall s' il',
+       feasible_set (removelast (d0 :: drest)) s' ->
+       is_indexed_elements (removelast (d0 :: drest)) il' s' ->
+       non_adjacent_in il' -> sum s' = max2 ->
+       index_lex_lt il2 il' \/ il2 = il') ->
+    max2 + x = max1 ->
+    index_lex_lt (il2 ++ [idx]) il1 ->
+    feasible_set ((d0 :: drest) ++ [x]) s' ->
+    is_indexed_elements ((d0 :: drest) ++ [x]) il' s' ->
+    non_adjacent_in il' ->
+    sum s' = max2 + x ->
+    index_lex_lt (il2 ++ [idx]) il' \/ il2 ++ [idx] = il'. 
+Proof. 
+Admitted.
+
+Lemma max_sum_lex_inv_eq_case : 
+  forall (l : list Z) (x d0 : Z) (drest ans1 il1 ans2 il2 : list Z) (max1 max2 idx : Z)
+    (Hlen :  Zlength (d0 :: drest) = idx)
+    (Hfull1 : max_sum_full_spec (d0 :: drest) max1 ans1)
+    (Hidx1 : is_indexed_elements (d0 :: drest) il1 ans1)
+    (Hgap1 : non_adjacent_in il1)
+    (Hlex1 : forall s' il',
+               feasible_set (d0 :: drest) s' ->
+               is_indexed_elements (d0 :: drest) il' s' ->
+               non_adjacent_in il' -> sum s' = max1 ->
+               index_lex_lt il1 il' \/ il1 = il')
+    (Hfull2 : max_sum_full_spec (removelast (d0 :: drest)) max2 ans2)
+    (Hidx2 : is_indexed_elements (removelast (d0 :: drest)) il2 ans2)
+    (Hgap2 : non_adjacent_in il2)
+    (Hlex2 : forall s' il',
+               feasible_set (removelast (d0 ::  drest)) s' ->
+               is_indexed_elements (removelast (d0 :: drest)) il' s' ->
+               non_adjacent_in il' -> sum s' = max2 ->
+               index_lex_lt il2 il' \/ il2 = il')
+    (Heq : max2 + x = max1)
+    (Hlex : index_lex_lt (il2 ++ [idx]) il1),
+  max_sum_lex_inv ((d0 :: drest) ++ [x]) (max2 + x) (ans2 ++ [x]) (il2 ++ [idx]) max1 ans1 il1 (idx + 1).
+Proof.
+  intros l x d0 drest ans1 il1 ans2 il2 max1 max2 idx Hlen Hfull1 Hidx1 Hgap1 Hlex1 Hfull2 Hidx2 Hgap2 Hlex2 Heq Hlex.
+  unfold max_sum_lex_inv.
+  repeat split. 
+
+  - rewrite Zlength_app. rewrite Hlen.  unfold Zlength; simpl; reflexivity.
+  - assert (Hspec1 := proj1 Hfull1).
+    assert (Hspec2 := proj1 Hfull2).
+    pose proof (max_value_spec_app (d0 :: drest) x max1 max2 Hspec1 Hspec2) as Hspec_app. 
+    assert (Hmax : Z.max max1 (max2 + x) = max2 + x).
+    {
+      rewrite Heq. 
+      apply Z.max_idempotent.
+    }
+    rewrite Hmax in Hspec_app.
+    exact Hspec_app.
+  - apply feasible_set_extend. apply (proj1 (proj2 Hfull2)).
+  - rewrite sum_app, sum_single. rewrite (proj2 (proj2 Hfull2)). reflexivity.
+  - apply is_indexed_elements_app.
+    + apply is_indexed_elements_extend; exact Hidx2.
+    + apply is_indexed_elements_cons.
+      * rewrite <- Hlen. apply Znth_error_snoc_last.
+      * apply is_indexed_elements_nil.
+  - apply sincr_extend_last. 
+    + apply (proj1 Hgap2).
+    + destruct il2 as [|i0 il2']. 
+      * left; reflexivity. 
+      * right.
+        assert (Hrem: Zlength (removelast (d0 ::  drest)) = idx - 1).
+        { rewrite Zlength_removelast. rewrite Hlen. reflexivity. discriminate. }
+        pose proof (is_indexed_elements_range _ _ _ Hidx2) as Hrange.
+        rewrite Forall_forall in Hrange.
+        assert (Hlast: In (last (i0 :: il2') 0) (i0 :: il2')) by (apply last_In; discriminate).
+        specialize (Hrange _ Hlast).
+        rewrite Hrem in Hrange. lia. 
+  - intros i j Hi Hj.
+    apply in_app_or in Hi; apply in_app_or in Hj.
+    destruct Hi as [Hi2 | Hi_eq]; destruct Hj as [Hj2 | Hj_eq].
+    + apply (proj2 Hgap2); tauto.
+    + apply in_singleton in Hj_eq; subst j.
+      assert (Hrem: Zlength (removelast (d0 :: drest)) = idx - 1).
+      { rewrite Zlength_removelast.  rewrite Hlen; reflexivity. discriminate. }
+      pose proof (is_indexed_elements_range _ _ _ Hidx2) as Hrange.
+      rewrite Forall_forall in Hrange; specialize (Hrange i Hi2).
+      rewrite Hrem in Hrange; lia.
+    + apply in_singleton in Hi_eq; subst i.
+      assert (Hrem: Zlength (removelast (d0 :: drest)) = idx - 1).
+      { rewrite Zlength_removelast.  rewrite Hlen; reflexivity. discriminate. }
+      pose proof (is_indexed_elements_range _ _ _ Hidx2) as Hrange.
+      rewrite Forall_forall in Hrange; specialize (Hrange j Hj2).
+      rewrite Hrem in Hrange; lia. 
+    + apply in_singleton in Hi_eq; apply in_singleton in Hj_eq; subst i j; lia. 
+  - intros s' il' Hfeas Hidx' Hnonadj Hsum.
+    apply (index_lex_preserve_eq_case d0 x drest ans1 il1 ans2 il2 max1 max2 idx s' il'
+             Hlen Hfull1 Hidx1 Hgap1 Hlex1 Hfull2 Hidx2 Hgap2 Hlex2 Heq Hlex 
+             Hfeas Hidx' Hnonadj Hsum).
+  - rewrite removelast_app_x. apply (proj1 Hfull1).
+  - rewrite removelast_app_x. apply (proj1 (proj2 Hfull1)).
+  - apply (proj2 (proj2 Hfull1)).
+  - rewrite removelast_app_x. exact Hidx1.
+  - apply (proj1 Hgap1).
+  - apply (proj2 Hgap1).
+  - rewrite removelast_app_x. apply Hlex1.
+Qed.
+
+Lemma index_lex_preserve_eq_nlex_case :
+  forall (d0 x : Z) (drest ans1 il1 ans2 il2 : list Z) (max1 max2 idx : Z)
+    (s' il' : list Z),
+    Zlength (d0 :: drest) = idx ->
+    max_sum_full_spec (d0 :: drest) max1 ans1 ->
+    is_indexed_elements (d0 :: drest) il1 ans1 ->
+    non_adjacent_in il1 ->
+    (forall s' il',
+       feasible_set (d0 :: drest) s' ->
+       is_indexed_elements (d0 :: drest) il' s' ->
+       non_adjacent_in il' -> sum s' = max1 ->
+       index_lex_lt il1 il' \/ il1 = il') ->
+    max_sum_full_spec (removelast (d0 :: drest)) max2 ans2 ->
+    is_indexed_elements (removelast (d0 :: drest)) il2 ans2 ->
+    non_adjacent_in il2 ->
+    (forall s' il',
+       feasible_set (removelast (d0 :: drest)) s' ->
+       is_indexed_elements (removelast (d0 :: drest)) il' s' ->
+       non_adjacent_in il' -> sum s' = max2 ->
+       index_lex_lt il2 il' \/ il2 = il') ->
+    max2 + x = max1 ->
+    ~ index_lex_lt (il2 ++ [idx]) il1 ->
+    feasible_set ((d0 ::  drest) ++ [x]) s' ->
+    is_indexed_elements ((d0 :: drest) ++ [x]) il' s' ->
+    non_adjacent_in il' ->
+    sum s' = max1 ->
+    index_lex_lt il1 il' \/ il1 = il'. 
+Proof. 
+Admitted.
+
+Lemma max_sum_lex_inv_eq_nlex_case :
+  forall (x d0 : Z) (drest ans1 il1 ans2 il2 : list Z) (max1 max2 idx : Z)
+    (Hlen : Zlength (d0 :: drest) = idx)
+    (Hfull1 : max_sum_full_spec (d0 :: drest) max1 ans1)
+    (Hidx1 :  is_indexed_elements (d0 :: drest) il1 ans1)
+    (Hgap1 : non_adjacent_in il1)
+    (Hlex1 : forall s' il',
+               feasible_set (d0 :: drest) s' ->
+               is_indexed_elements (d0 :: drest) il' s' ->
+               non_adjacent_in il' -> sum s' = max1 ->
+               index_lex_lt il1 il' \/ il1 = il')
+    (Hfull2 : max_sum_full_spec (removelast (d0 :: drest)) max2 ans2)
+    (Hidx2 : is_indexed_elements (removelast (d0 :: drest)) il2 ans2)
+    (Hgap2 : non_adjacent_in il2)
+    (Hlex2 : forall s' il',
+               feasible_set (removelast (d0 :: drest)) s' ->
+               is_indexed_elements (removelast (d0 :: drest)) il' s' ->
+               non_adjacent_in il' -> sum s' = max2 ->
+               index_lex_lt il2 il' \/ il2 = il')
+    (Heq : max2 + x = max1)
+    (Hnlex :  ~ index_lex_lt (il2 ++ [idx]) il1),
+  max_sum_lex_inv ((d0 :: drest) ++ [x]) max1 ans1 il1 max1 ans1 il1 (idx + 1).
+Proof.
+  intros x d0 drest ans1 il1 ans2 il2 max1 max2 idx Hlen Hfull1 Hidx1 Hgap1 Hlex1 Hfull2 Hidx2 Hgap2 Hlex2 Heq Hnlex.
+  unfold max_sum_lex_inv. 
+  repeat split.
+  - rewrite Zlength_app. rewrite Hlen; unfold Zlength; tauto.
+  - assert (Hspec1 := proj1 Hfull1).
+    assert (Hspec2 := proj1 Hfull2).
+    pose proof (max_value_spec_app (d0 :: drest) x max1 max2 Hspec1 Hspec2) as Hspec_app.
+    assert (Hmax : Z.max max1 (max2 + x) = max2 + x).
+    {
+      rewrite Heq. 
+      apply Z.max_idempotent.
+    }
+    rewrite Hmax in Hspec_app.
+    rewrite Heq in Hspec_app.
+    apply Hspec_app.
+  - apply feasible_set_app_x_l.
+    apply (proj1 (proj2 Hfull1)).
+  - apply (proj2 (proj2 Hfull1)).
+  - apply is_indexed_elements_prefix_extend.
+    exact Hidx1.
+  - apply (proj1 Hgap1).
+  - apply (proj2 Hgap1).
+  - intros s' il' Hfeas Hidx' Hnonadj Hsum.
+    apply (index_lex_preserve_eq_nlex_case d0 x drest ans1 il1 ans2 il2 max1 max2 idx s' il'
+             Hlen Hfull1 Hidx1 Hgap1 Hlex1 Hfull2 Hidx2 Hgap2 Hlex2 Heq Hnlex
+             Hfeas Hidx' Hnonadj Hsum).
+  - rewrite removelast_app_x.  apply (proj1 Hfull1).
+  - rewrite removelast_app_x.  apply (proj1 (proj2 Hfull1)).
+  - apply (proj2 (proj2 Hfull1)).
+  - rewrite removelast_app_x. exact Hidx1.
+  - apply (proj1 Hgap1).
+  - apply (proj2 Hgap1).
+  - rewrite removelast_app_x. exact Hlex1.
+Qed.
+
 (** Level 4: Prove that the modified algorithm returns the lexicographically minimal optimal solution *)
 Theorem max_sum_lex_correct :
   forall l,
     Hoare (max_sum_lex l)
       (fun '(m, s, il) => lex_min_spec l m s il).
 Proof.
-Admitted.
+  intros l.
+  unfold max_sum_lex.
+  eapply Hoare_bind.
+  - eapply Hoare_list_iter with
+      (I := fun done st =>
+        match st with
+        | (max1, ans1, il1, max2, ans2, il2, idx) =>
+            max_sum_lex_inv done max1 ans1 il1 max2 ans2 il2 idx
+        end).
+    + repeat split.
+      * apply max_value_spec_nil.
+      * apply feasible_set_nil_intro.
+      * apply is_indexed_elements_nil.
+      * tauto.
+      * intros. right. apply proof_il'_nil with s'; tauto.
+    + intros x done st.
+      destruct st as [[[[[[max1 ans1] il1] max2] ans2] il2] idx].
+      intros [Hlen [Hfull1 [Hidx1 [Hgap1 [Hlex1 Hrem]]]]].
+
+      destruct done as [|d0 drest].
+      * destruct Hrem as [-> [-> ->]].
+        apply Hoare_choice.
+        -- eapply Hoare_assume_bind.
+           intros Hgt.
+           apply Hoare_ret.
+
+           assert (Hfeas1 : feasible_set [] ans1) by (apply (proj1 (proj2 Hfull1))).
+           apply feasible_set_nil in Hfeas1. subst ans1.
+           simpl in Hgt.  (* now Hgt : x > max1 *)
+           assert (Hsum1 : sum [] = max1) by (apply (proj2 (proj2 Hfull1))); simpl in Hsum1.
+           subst max1.  (* now max1 = 0 *)
+           apply is_indexed_elements_nil_inv_r in Hidx1. subst il1.
+           assert (Hidx0 : idx = 0). { apply idx_eq_zero. apply Hlen. }
+           subst idx. simpl. rewrite Hidx0.
+           apply max_sum_lex_inv_single_positive; tauto.
+        -- apply Hoare_choice.
+           ++ eapply Hoare_assume_bind.
+              intros Hlt; simpl in Hlt.
+              apply Hoare_ret. simpl.
+              apply max_sum_lex_inv_single_case; tauto.
+           ++ eapply Hoare_assume_bind.
+              intros Heq; simpl in Heq.
+              apply Hoare_choice.
+              ** apply Hoare_assume_bind.
+                 intros Hlt.
+                 apply Hoare_ret; simpl.
+                 (* 此时 Hlt 内存在矛盾 *)
+                 apply max_sum_lex_inv_contradiction_case; tauto.
+              ** apply Hoare_assume_bind.
+                 intros Hnlt.
+                 apply Hoare_ret; simpl.
+                 apply max_sum_lex_inv_valid_case; tauto.
+      * destruct Hrem as [Hfull2 [Hidx2 [Hgap2 Hlex2]]].
+        apply Hoare_choice.
+        -- eapply Hoare_assume_bind.
+           intros Hgt.
+           apply Hoare_ret.
+           apply max_sum_lex_inv_extend_case; tauto.
+        -- apply Hoare_choice.
+           ++ eapply Hoare_assume_bind.
+              intros Hlt.
+              apply Hoare_ret.
+              rewrite <- Hlen.
+              apply max_sum_lex_inv_preserve_when_not_taken
+              with (l := (d0 :: drest))
+                   (x := x)
+                   (max1 := max1)
+                   (max2 := max2)
+                   (ans1 := ans1)
+                   (ans2 := ans2)
+                   (il1 := il1). discriminate. tauto. tauto. tauto. tauto. tauto. tauto.
+           ++ eapply Hoare_assume_bind.
+              intros Heq.
+              apply Hoare_choice.
+              ** eapply Hoare_assume_bind.
+                 intros Hlex.
+                 apply Hoare_ret.
+                 apply max_sum_lex_inv_eq_case; tauto.
+              ** eapply Hoare_assume_bind.
+                 intros Hnlex.
+                 apply Hoare_ret.
+                 apply max_sum_lex_inv_eq_nlex_case
+                 with 
+                   (x := x)
+                   (max1 := max1)
+                   (max2 := max2)
+                   (ans1 := ans1)
+                   (ans2 := ans2)
+                   (il1 := il1)
+                   (il2 := il2); tauto.
+  - intros a Hinv.
+    destruct a as [[[[[[max1 ans1] il1] max2] ans2] il2] idx].
+    destruct Hinv as [Hlen [Hfull [Hidx [Hgap [Hlex _]]]]].
+    unfold lex_min_spec.
+    apply Hoare_ret.
+    tauto.
+Qed.
